src/NonEmptyList.v
@@ -1,0 +1,24 @@
+Set Implicit Arguments.
+
+Require Import List.
+
+Section NEList.
+
+  Variable A:Type.
+
+  Definition nelist := (A * list A)%type.
+
+  Definition single x : nelist := (x, nil).
+
+  Definition append (l1 l2: nelist) : nelist :=
+    let (x, xs) := l1 in
+    let (y, ys) := l2 in
+    (x, xs ++ cons y ys).
+
+  Definition hd (l:nelist) : A :=
+    let (x, _) := l in x.
+
+  Definition tl (l:nelist) : list A :=
+    let (_, xs) := l in xs.
+
+End NEList.
